Logic/Propositional/Superintuitionistic/Kripke/DP.lean
@@ -1,6 +1,7 @@
 import Logic.Logic.Disjunctive
-import Logic.Propositional.Superintuitionistic.Kripke.Soundness
 import Logic.Propositional.Superintuitionistic.Kripke.Completeness
+
+-- TODO: 証明自体は通っているがコードが雑なためそのうちリファクタリングする
 
 namespace LO.Propositional.Superintuitionistic
 
@@ -12,109 +13,134 @@ namespace Kripke
 variable {α} [Inhabited α] [DecidableEq α] [Encodable α]
 variable {p q : Formula α}
 
-abbrev IntDPCounterexampleFrame (F₁ : Frame.{u}) (F₂ : Frame.{u}) (w₁ : F₁.World) (w₂ : F₂.World) : Frame where
+abbrev IntDPCounterexampleFrame (F₁ : Kripke.Frame) (F₂ : Kripke.Frame) (w₁ : F₁.World) (w₂ : F₂.World) : Kripke.Frame where
   World := Unit ⊕ F₁.World ⊕ F₂.World;
-  Rel w v :=
-    match w, v with
+  Rel x y :=
+    match x, y with
     | (Sum.inl _), (Sum.inl _) => True
-    | (Sum.inl _), (Sum.inr $ Sum.inl v) => w₁ ≺ v
-    | (Sum.inl _), (Sum.inr $ Sum.inr v) => w₂ ≺ v
-    | (Sum.inr $ Sum.inl w), (Sum.inr $ Sum.inl v) => w ≺ v
-    | (Sum.inr $ Sum.inr w), (Sum.inr $ Sum.inr v) => w ≺ v
+    | (Sum.inl _), (Sum.inr $ Sum.inl y) => F₁.Rel w₁ y
+    | (Sum.inl _), (Sum.inr $ Sum.inr y) => F₂.Rel w₂ y
+    | (Sum.inr $ Sum.inl x), (Sum.inr $ Sum.inl y) => F₁.Rel x y
+    | (Sum.inr $ Sum.inr x), (Sum.inr $ Sum.inr y) => F₂.Rel x y
     | _, _ => False
-  Rel_refl := by
-    simp only [Reflexive, Sum.forall, forall_const, true_and];
-    constructor;
-    . exact F₁.Rel_refl;
-    . exact F₂.Rel_refl;
-  Rel_trans := by
-    simp only [Transitive, Sum.forall, forall_true_left, imp_self, forall_const, true_and, IsEmpty.forall_iff, implies_true, and_true, and_self, imp_false];
-    constructor;
-    . constructor;
-      . intro _ _; apply F₁.Rel_trans;
-      . intro _ _; apply F₂.Rel_trans;
-    . constructor;
-      . intro _ _; apply F₁.Rel_trans;
-      . intro _ _; apply F₂.Rel_trans;
-  Rel_antisymm := by
-    simp only [Antisymmetric, Sum.forall, forall_true_left, forall_const, IsEmpty.forall_iff, implies_true, and_self, imp_false, Sum.inr.injEq, true_and, Sum.inl.injEq, and_true];
-    constructor;
-    . exact F₁.Rel_antisymm;
-    . exact F₂.Rel_antisymm;
 
-abbrev IntDPCounterexampleModel (M₁ : Model α) (M₂ : Model α) (w₁ : M₁.World) (w₂ : M₂.World) : Model α where
+lemma IntDPCounterexampleFrame.reflexive
+  {F₁ : Kripke.Frame} {F₂ : Kripke.Frame}
+  {w₁ : F₁.World} {w₂ : F₂.World}
+  (F₁_refl : Reflexive F₁.Rel) (F₂_refl : Reflexive F₂.Rel)
+  : Reflexive (IntDPCounterexampleFrame F₁ F₂ w₁ w₂).Rel := by
+  simp only [Reflexive, Sum.forall, forall_const, true_and];
+  constructor;
+  . exact F₁_refl;
+  . exact F₂_refl;
+
+lemma IntDPCounterexampleFrame.transitive
+  {F₁ : Kripke.Frame} {F₂ : Kripke.Frame}
+  {w₁ : F₁.World} {w₂ : F₂.World}
+  (F₁_trans : Transitive F₁.Rel) (F₂_trans : Transitive F₂.Rel)
+  : Transitive (IntDPCounterexampleFrame F₁ F₂ w₁ w₂).Rel := by
+  simp only [Transitive, Sum.forall, forall_true_left, imp_self, forall_const, true_and, IsEmpty.forall_iff, implies_true, and_true, and_self, imp_false];
+  constructor;
+  . constructor;
+    . intro _ _; apply F₁_trans;
+    . intro _ _; apply F₂_trans;
+  . constructor;
+    . intro _ _; apply F₁_trans;
+    . intro _ _; apply F₂_trans;
+
+lemma IntDPCounterexampleFrame.antisymmetric
+  {F₁ : Kripke.Frame} {F₂ : Kripke.Frame}
+  {w₁ : F₁.World} {w₂ : F₂.World}
+  (F₁_antisymm : Antisymmetric F₁.Rel) (F₂_antisymm : Antisymmetric F₂.Rel)
+  : Antisymmetric (IntDPCounterexampleFrame F₁ F₂ w₁ w₂).Rel := by
+  simp only [Antisymmetric, Sum.forall, forall_true_left, forall_const, IsEmpty.forall_iff, implies_true, and_self, imp_false, Sum.inr.injEq, true_and, Sum.inl.injEq, and_true];
+  constructor;
+  . exact F₁_antisymm;
+  . exact F₂_antisymm;
+
+abbrev IntDPCounterexampleModel (M₁ : Kripke.Model α) (M₂ : Kripke.Model α) (w₁ : M₁.World) (w₂ : M₂.World) : Kripke.Model α where
   Frame := IntDPCounterexampleFrame M₁.Frame M₂.Frame w₁ w₂;
   Valuation w a :=
     match w with
     | Sum.inr $ Sum.inl w => M₁.Valuation w a
     | Sum.inr $ Sum.inr w => M₂.Valuation w a
     | _ => False
-  hereditary := by
-    simp only [Sum.forall, imp_false, not_false_eq_true, implies_true, forall_true_left, forall_const, IsEmpty.forall_iff, and_self, and_true, true_and];
-    constructor;
-    . intro _ _; apply M₁.hereditary;
-    . intro _ _; apply M₂.hereditary;
 
-variable {M₁ : Model α} {M₂ : Model α}
+lemma IntDPCounterexampleModel.atomic_hereditary
+  {M₁ : Kripke.Model α} {M₂ : Kripke.Model α}
+  {w₁ : M₁.World} {w₂ : M₂.World}
+  (M₁_hered : M₁.Valuation.atomic_hereditary) (M₂_hered : M₂.Valuation.atomic_hereditary)
+  : (IntDPCounterexampleModel M₁ M₂ w₁ w₂).Valuation.atomic_hereditary := by
+  simp;
+  constructor;
+  . apply M₁_hered;
+  . apply M₂_hered;
+
+variable {M₁ : Kripke.Model α} {M₂ : Kripke.Model α}
 
 lemma satisfies_left_on_IntDPCounterexampleModel :
   (Satisfies M₁ w p) ↔ (Satisfies (IntDPCounterexampleModel M₁ M₂ w₁ w₂) (Sum.inr $ Sum.inl w) p) := by
-  -- ((M₁, w) ⊧ p) ↔ ((IntDPCounterexampleModel M₁ M₂ w₁ w₂, (Sum.inr $ Sum.inl w : (Unit ⊕ W₁ ⊕ W₂))) ⊧ p) := by
   induction p using rec' generalizing w with
   | himp p q ihp ihq =>
     constructor;
-    . simp only [Satisfies.imp_def];
-      intro h X hWX hp;
-      obtain ⟨x, hx, ex⟩ : ∃ x, w ≺ x ∧ (Sum.inr $ Sum.inl x) = X := by
+    . intro hpq X hWX hp;
+      obtain ⟨x, hx, ex⟩ : ∃ x, (M₁.Frame.Rel w x) ∧ (Sum.inr $ Sum.inl x) = X := by
         replace hWX : (IntDPCounterexampleModel M₁ M₂ w₁ w₂).Frame.Rel _ X := hWX;
         simp [IntDPCounterexampleFrame] at hWX;
         split at hWX;
         all_goals simp_all;
       subst ex;
-      exact ihq.mp $ h hx $ ihp.mpr hp;
-    . simp only [Satisfies.imp_def];
-      intro h v hv hp;
-      exact ihq.mpr $ h (by simpa [IntDPCounterexampleModel]) $ ihp.mp hp;
+      exact ihq.mp $ hpq hx $ ihp.mpr hp;
+    . intro h v Rwv hp;
+      apply @ihq v |>.mpr $ h (by simpa) $ ihp.mp hp;
   | _ => simp_all [IntDPCounterexampleModel, Satisfies.iff_models, Satisfies];
 
 lemma satisfies_right_on_IntDPCounterexampleModel :
   (Satisfies M₂ w p) ↔ (Satisfies (IntDPCounterexampleModel M₁ M₂ w₁ w₂) (Sum.inr $ Sum.inr w) p) := by
-  -- : ((M₂, w) ⊧ p) ↔ ((IntDPCounterexampleModel M₁ M₂ w₁ w₂, (Sum.inr $ Sum.inr w : (Unit ⊕ W₁ ⊕ W₂))) ⊧ p) := by
   induction p using rec' generalizing w with
   | himp p q ihp ihq =>
     constructor;
-    . simp only [Satisfies.imp_def];
-      intro h X hWX hp;
-      obtain ⟨x, hx, ex⟩ : ∃ x, w ≺ x ∧ (Sum.inr $ Sum.inr x) = X := by
+    . intro h X hWX hp;
+      obtain ⟨x, hx, ex⟩ : ∃ x, (M₂.Frame.Rel w x) ∧ (Sum.inr $ Sum.inr x) = X := by
         replace hWX : (IntDPCounterexampleModel M₁ M₂ w₁ w₂).Frame.Rel _ X := hWX;
         simp [IntDPCounterexampleFrame] at hWX;
         split at hWX;
         all_goals simp_all;
       subst ex;
       exact ihq.mp $ h hx $ ihp.mpr hp;
-    . simp only [Satisfies.imp_def];
-      intro h v hv hp;
-      exact ihq.mpr $ h (by simpa [IntDPCounterexampleModel]) $ ihp.mp hp;
+    . intro h v Rwv hp;
+      exact ihq.mpr $ h (by simpa) $ ihp.mp hp;
   | _ => simp_all [IntDPCounterexampleModel, Satisfies.iff_models, Satisfies];
 
 theorem disjunctive_int : 𝐈𝐧𝐭 ⊢! p ⋎ q → 𝐈𝐧𝐭 ⊢! p ∨ 𝐈𝐧𝐭 ⊢! q := by
   contrapose;
   intro hC; push_neg at hC;
   have ⟨hnp, hnq⟩ := hC;
-  obtain ⟨Fp, _, Vp, hVp, wp, hp⟩ := by simpa [ValidOnFrameClass, ValidOnFrame, ValidOnModel] using not_imp_not.mpr complete! hnp;
-  obtain ⟨Fq, _, Vq, hVq, wq, hq⟩ := by simpa [ValidOnFrameClass, ValidOnFrame, ValidOnModel] using not_imp_not.mpr complete! hnq;
-  apply (not_imp_not.mpr sound!);
-
-  simp [ValidOnFrameClass, ValidOnFrame, ValidOnModel];
-  let M : Model α := IntDPCounterexampleModel ⟨Fp, Vp, hVp⟩ ⟨Fq, Vq, hVq⟩ wp wq;
-  existsi M.Frame;
+  obtain ⟨Fp, Fp_refl, Fp_trans, Vp, Vp_hered, wp, hp⟩ := by simpa [Semantics.Realize, ValidOnFrame, ValidOnModel] using not_imp_not.mpr (@Kripke.Int_Complete α _ _ |>.complete) hnp;
+  obtain ⟨Fq, Fq_refl, Fq_trans, Vq, Vq_hered, wq, hq⟩ := by simpa [Semantics.Realize, ValidOnFrame, ValidOnModel] using not_imp_not.mpr (@Kripke.Int_Complete α _ _ |>.complete) hnq;
+  apply (not_imp_not.mpr Int_sound.sound);
+  simp [Semantics.Realize, ValidOnFrame, ValidOnModel, Satisfies];
+  use (IntDPCounterexampleFrame Fp Fq wp wq);
+  refine ⟨IntDPCounterexampleFrame.reflexive Fp_refl Fq_refl, IntDPCounterexampleFrame.transitive Fp_trans Fq_trans, ?_⟩;
+  use (IntDPCounterexampleModel ⟨Fp, Vp⟩ ⟨Fq, Vq⟩ wp wq).Valuation;
   constructor;
-  . apply iff_definability_memAxiomSetFrameClass AxiomSet.EFQ.definability |>.mpr;
-    trivial;
-  . existsi M.Valuation, M.hereditary, Sum.inl ();
+  . exact @IntDPCounterexampleModel.atomic_hereditary α ⟨Fp, Vp⟩ ⟨Fq, Vq⟩ wp wq Vp_hered Vq_hered;
+  . use (Sum.inl ());
     constructor;
-    . exact not_imp_not.mpr (Satisfies.formula_hereditary (by apply Fp.Rel_refl)) $ satisfies_left_on_IntDPCounterexampleModel.not.mp hp;
-    . exact not_imp_not.mpr (Satisfies.formula_hereditary (by apply Fq.Rel_refl)) $ satisfies_right_on_IntDPCounterexampleModel.not.mp hq;
+    . exact not_imp_not.mpr
+        (Satisfies.formula_hereditary
+          (M := IntDPCounterexampleModel ⟨Fp, Vp⟩ ⟨Fq, Vq⟩ wp wq)
+          (IntDPCounterexampleModel.atomic_hereditary Vp_hered Vq_hered)
+          (IntDPCounterexampleFrame.transitive Fp_trans Fq_trans)
+          (w := Sum.inl ()) (w' := Sum.inr $ Sum.inl wp) (by aesop))
+        $ satisfies_left_on_IntDPCounterexampleModel |>.not.mp hp;
+    . exact not_imp_not.mpr
+        (Satisfies.formula_hereditary
+          (M := IntDPCounterexampleModel ⟨Fp, Vp⟩ ⟨Fq, Vq⟩ wp wq)
+          (IntDPCounterexampleModel.atomic_hereditary Vp_hered Vq_hered)
+          (IntDPCounterexampleFrame.transitive Fp_trans Fq_trans)
+          (w := Sum.inl ()) (w' := Sum.inr $ Sum.inr wq) (by aesop))
+        $ satisfies_right_on_IntDPCounterexampleModel |>.not.mp hq;
 
 instance : Disjunctive (𝐈𝐧𝐭 : DeductionParameter α) := ⟨disjunctive_int⟩
 
